silveroak-opentitan/aes/Acorn/AES256Equivalence.v
@@ -1,0 +1,160 @@
+(****************************************************************************)
+(* Copyright 2020 The Project Oak Authors                                   *)
+(*                                                                          *)
+(* Licensed under the Apache License, Version 2.0 (the "License")           *)
+(* you may not use this file except in compliance with the License.         *)
+(* You may obtain a copy of the License at                                  *)
+(*                                                                          *)
+(*     http://www.apache.org/licenses/LICENSE-2.0                           *)
+(*                                                                          *)
+(* Unless required by applicable law or agreed to in writing, software      *)
+(* distributed under the License is distributed on an "AS IS" BASIS,        *)
+(* WITHOUT WARRANTIES OR CONDITIONS OF ANY KIND, either express or implied. *)
+(* See the License for the specific language governing permissions and      *)
+(* limitations under the License.                                           *)
+(****************************************************************************)
+
+Require Import Coq.Vectors.Vector.
+Require Import ExtLib.Structures.Monads.
+Require Import Cava.ListUtils.
+Require Import Cava.VectorUtils.
+Require Import Cava.Acorn.Acorn.
+Require Import Cava.Acorn.MonadFacts.
+Require Import Cava.Acorn.Identity.
+
+Require Import AesSpec.AES256.
+Require Import AesSpec.StateTypeConversions.
+Require Import AesSpec.CipherProperties.
+Require Import AcornAes.AddRoundKey.
+Require Import AcornAes.AddRoundKeyEquivalence.
+Require Import AcornAes.CipherRound.
+Require Import AcornAes.CipherEquivalence.
+Require Import AcornAes.Common.
+Import Common.Notations.
+
+Axiom sub_bytes : forall {signal} {semantics : Cava signal} {monad : Monad cava},
+    signal Bit -> signal state -> cava (signal state).
+Axiom shift_rows : forall {signal} {semantics : Cava signal} {monad : Monad cava},
+    signal Bit -> signal state -> cava (signal state).
+Axiom mix_columns : forall {signal} {semantics : Cava signal} {monad : Monad cava},
+    signal Bit -> signal state -> cava (signal state).
+
+Axiom sub_bytes_equiv :
+ forall st : t bool 128,
+   from_cols_bitvecs
+     (combinational (sub_bytes false (to_cols_bitvecs st))) = AES256.sub_bytes st.
+Axiom shift_rows_equiv :
+  forall st : t bool 128,
+    from_cols_bitvecs
+      (combinational (shift_rows false (to_cols_bitvecs st))) = AES256.shift_rows st.
+Axiom mix_columns_equiv :
+  forall st : t bool 128,
+    from_cols_bitvecs
+      (combinational (mix_columns false (to_cols_bitvecs st))) = AES256.mix_columns st.
+Axiom inv_sub_bytes_equiv :
+ forall st : t bool 128,
+   from_cols_bitvecs
+     (combinational (sub_bytes true (to_cols_bitvecs st))) = inv_sub_bytes st.
+Axiom inv_shift_rows_equiv :
+  forall st : t bool 128,
+    from_cols_bitvecs
+      (combinational (shift_rows true (to_cols_bitvecs st))) = inv_shift_rows st.
+Axiom inv_mix_columns_equiv :
+  forall st : t bool 128,
+    from_cols_bitvecs
+      (combinational (mix_columns true (to_cols_bitvecs st))) = inv_mix_columns st.
+
+Hint Resolve add_round_key_equiv sub_bytes_equiv shift_rows_equiv
+     mix_columns_equiv inv_sub_bytes_equiv inv_shift_rows_equiv
+     inv_mix_columns_equiv : subroutines_equiv.
+
+Definition full_cipher {signal} {semantics : Cava signal} {monad : Monad cava}
+  : signal Bit -> signal key -> signal key -> list (signal key) -> signal state
+    -> cava (signal state) :=
+  cipher sub_bytes shift_rows mix_columns add_round_key.
+
+Lemma full_cipher_equiv
+      (is_decrypt : bool)
+      (first_key last_key : combType key) (middle_keys : list (combType key))
+      (input : combType state) :
+  combinational
+    (full_cipher is_decrypt first_key last_key middle_keys input)
+  = to_cols_bitvecs
+      ((if is_decrypt then aes256_decrypt else aes256_encrypt)
+         (from_cols_bitvecs first_key) (from_cols_bitvecs last_key)
+         (List.map from_cols_bitvecs middle_keys) (from_cols_bitvecs input)).
+Proof.
+  cbv [full_cipher].
+
+  destruct is_decrypt.
+  { (* decryption *)
+    rewrite inverse_cipher_equiv. cbv [aes256_decrypt].
+
+    (* Change key and state representations so they match *)
+    erewrite equivalent_inverse_cipher_change_state_rep
+      by eapply to_cols_bitvecs_from_cols_bitvecs.
+    erewrite equivalent_inverse_cipher_change_key_rep
+      with (projkey:=to_cols_bitvecs)
+           (middle_keys_alt:=List.map from_cols_bitvecs middle_keys)
+      by (apply to_cols_bitvecs_from_cols_bitvecs ||
+          (rewrite List.map_map; apply ListUtils.map_id_ext;
+           intros; autorewrite with conversions; reflexivity)).
+
+    (* Prove that ciphers are equivalent because all subroutines are
+       equivalent *)
+    f_equal.
+    eapply equivalent_inverse_cipher_subroutine_ext;
+      eauto with subroutines_equiv. }
+  { (* encryption *)
+    rewrite cipher_equiv. cbv [aes256_encrypt].
+
+    (* Change key and state representations so they match *)
+    erewrite cipher_change_state_rep
+      by eapply to_cols_bitvecs_from_cols_bitvecs.
+    erewrite cipher_change_key_rep
+      with (projkey:=to_cols_bitvecs)
+           (middle_keys_alt:=List.map from_cols_bitvecs middle_keys)
+      by (apply to_cols_bitvecs_from_cols_bitvecs ||
+          (rewrite List.map_map; apply ListUtils.map_id_ext;
+           intros; autorewrite with conversions; reflexivity)).
+
+    (* Prove that ciphers are equivalent because all subroutines are
+       equivalent *)
+    f_equal.
+    eapply cipher_subroutine_ext; eauto with subroutines_equiv. }
+Qed.
+
+Local Open Scope monad_scope.
+
+Lemma decrypt_middle_keys_equiv (middle_keys : list (combType key)) :
+  List.map (fun k => from_cols_bitvecs (combinational (mix_columns true k)))
+           (List.rev middle_keys) =
+  List.map inv_mix_columns (List.rev (List.map from_cols_bitvecs middle_keys)).
+Proof.
+  rewrite !List.map_rev. f_equal.
+  rewrite List.map_map. apply List.map_ext; intro x.
+  rewrite <-(to_cols_bitvecs_from_cols_bitvecs x).
+  rewrite inv_mix_columns_equiv.
+  autorewrite with conversions; reflexivity.
+Qed.
+
+Lemma full_cipher_inverse
+      (first_key last_key : combType key) (middle_keys : list (combType key))
+      (input : combType state) :
+  let decrypt_middle_keys :=
+      List.map (fun k => combinational (mix_columns true k)) (List.rev middle_keys) in
+  combinational
+    ((full_cipher false first_key last_key middle_keys >=>
+      full_cipher true last_key first_key decrypt_middle_keys) input) = input.
+Proof.
+  cbv [mcompose]. simpl_ident.
+  rewrite !full_cipher_equiv.
+  autorewrite with conversions.
+  rewrite List.map_map, decrypt_middle_keys_equiv.
+  rewrite aes256_decrypt_encrypt.
+  autorewrite with conversions.
+  reflexivity.
+Qed.
+
+Redirect "FullCipherEquiv_Assumptions" Print Assumptions full_cipher_equiv.
+Redirect "FullCipherInverse_Assumptions" Print Assumptions full_cipher_inverse.
