silveroak-opentitan/aes/Acorn/CipherEquivalence.v
@@ -29,21 +29,24 @@ Section WithSubroutines.
   Local Notation byte := (t bool 8).
   Local Notation state := (t (t byte 4) 4) (only parsing).
   Local Notation key := (t (t byte 4) 4) (only parsing).
-  Context (sub_bytes:     state -> ident state)
-          (shift_rows:    state -> ident state)
-          (mix_columns:   state -> ident state)
+  Context (sub_bytes:     bool -> state -> ident state)
+          (shift_rows:    bool -> state -> ident state)
+          (mix_columns:   bool -> state -> ident state)
           (add_round_key : key -> state -> ident state).
 
-  Let sub_bytes' : state -> state := (fun st => unIdent (sub_bytes st)).
-  Let shift_rows' : state -> state := (fun st => unIdent (shift_rows st)).
-  Let mix_columns' : state -> state := (fun st => unIdent (mix_columns st)).
+  Let sub_bytes' : state -> state := (fun st => unIdent (sub_bytes false st)).
+  Let shift_rows' : state -> state := (fun st => unIdent (shift_rows false st)).
+  Let mix_columns' : state -> state := (fun st => unIdent (mix_columns false st)).
+  Let inv_sub_bytes' : state -> state := (fun st => unIdent (sub_bytes true st)).
+  Let inv_shift_rows' : state -> state := (fun st => unIdent (shift_rows true st)).
+  Let inv_mix_columns' : state -> state := (fun st => unIdent (mix_columns true st)).
   (* Note: argument order is switched for spec *)
   Let add_round_key' : state -> key -> state :=
     (fun st k => unIdent (add_round_key k st)).
 
   Lemma cipher_equiv
         (first_key last_key : key) (middle_keys : list key) (input : state) :
-    let cipher := (cipher sub_bytes shift_rows mix_columns add_round_key) in
+    let cipher := (cipher sub_bytes shift_rows mix_columns add_round_key false) in
     let cipher_spec := (Cipher.cipher _ _ add_round_key'
                                       sub_bytes' shift_rows' mix_columns') in
     unIdent (cipher first_key last_key middle_keys input)
@@ -56,17 +59,16 @@ Section WithSubroutines.
     intros; subst. reflexivity.
   Qed.
 
-  (* If we assume all the subroutines are the inverse operations, we get the
-     equivalent inverse cipher *)
   Lemma inverse_cipher_equiv
         (first_key last_key : key) (middle_keys : list key) (input : state) :
-    let cipher := (cipher sub_bytes shift_rows mix_columns add_round_key) in
+    let cipher := (cipher sub_bytes shift_rows mix_columns add_round_key true) in
     let cipher_spec := (Cipher.equivalent_inverse_cipher
-                          _ _ add_round_key' sub_bytes' shift_rows' mix_columns') in
+                          _ _ add_round_key'
+                          inv_sub_bytes' inv_shift_rows' inv_mix_columns') in
     unIdent (cipher first_key last_key middle_keys input)
     = cipher_spec first_key last_key middle_keys input.
   Proof.
-    cbv zeta. subst sub_bytes' shift_rows' mix_columns' add_round_key'.
+    cbv zeta. subst inv_sub_bytes' inv_shift_rows' inv_mix_columns' add_round_key'.
     cbv [cipher cipher_round Cipher.equivalent_inverse_cipher].
     cbn [mcompose bind ret Monad_ident unIdent].
     repeat (f_equal; [ ]). rewrite foldLM_ident_fold_left.
