silveroak-opentitan/aes/Spec/CipherProperties.v
@@ -1,0 +1,158 @@
+(****************************************************************************)
+(* Copyright 2020 The Project Oak Authors                                   *)
+(*                                                                          *)
+(* Licensed under the Apache License, Version 2.0 (the "License")           *)
+(* you may not use this file except in compliance with the License.         *)
+(* You may obtain a copy of the License at                                  *)
+(*                                                                          *)
+(*     http://www.apache.org/licenses/LICENSE-2.0                           *)
+(*                                                                          *)
+(* Unless required by applicable law or agreed to in writing, software      *)
+(* distributed under the License is distributed on an "AS IS" BASIS,        *)
+(* WITHOUT WARRANTIES OR CONDITIONS OF ANY KIND, either express or implied. *)
+(* See the License for the specific language governing permissions and      *)
+(* limitations under the License.                                           *)
+(****************************************************************************)
+
+Require Import Coq.Lists.List.
+Require Import Cava.ListUtils.
+Require Import AesSpec.Cipher.
+
+Section ChangeRepresentation.
+  Context (state state_alt key key_alt : Type)
+          (projkey : key_alt -> key)
+          (to_state_alt : state -> state_alt)
+          (from_state_alt : state_alt -> state)
+          (add_round_key : state -> key -> state)
+          (sub_bytes shift_rows mix_columns : state -> state)
+          (inv_sub_bytes inv_shift_rows inv_mix_columns : state -> state).
+  Context (from_state_alt_to_state_alt : forall st, from_state_alt (to_state_alt st) = st).
+
+  Lemma cipher_change_key_rep first_key last_key middle_keys
+        first_key_alt last_key_alt middle_keys_alt input :
+    projkey first_key_alt = first_key ->
+    projkey last_key_alt = last_key ->
+    map projkey middle_keys_alt = middle_keys ->
+    cipher state key add_round_key sub_bytes shift_rows mix_columns
+           first_key last_key middle_keys input
+    = cipher state key_alt (fun st k => add_round_key st (projkey k))
+             sub_bytes shift_rows mix_columns first_key_alt last_key_alt
+             middle_keys_alt input.
+  Proof.
+    intros; subst; cbv [cipher].
+    repeat (f_equal; [ ]). rewrite fold_left_map.
+    reflexivity.
+  Qed.
+
+  Lemma equivalent_inverse_cipher_change_key_rep first_key last_key middle_keys
+        first_key_alt last_key_alt middle_keys_alt input :
+    projkey first_key_alt = first_key ->
+    projkey last_key_alt = last_key ->
+    map projkey middle_keys_alt = middle_keys ->
+    equivalent_inverse_cipher
+      state key add_round_key
+      inv_sub_bytes inv_shift_rows inv_mix_columns
+      first_key last_key middle_keys input
+    = equivalent_inverse_cipher
+        state key_alt (fun st k => add_round_key st (projkey k))
+        inv_sub_bytes inv_shift_rows inv_mix_columns first_key_alt last_key_alt
+        middle_keys_alt input.
+  Proof.
+    intros; subst; cbv [equivalent_inverse_cipher].
+    repeat (f_equal; [ ]). rewrite !fold_left_map.
+    reflexivity.
+  Qed.
+
+  Lemma cipher_change_state_rep first_key last_key middle_keys
+        input :
+    cipher state key add_round_key sub_bytes shift_rows mix_columns
+           first_key last_key middle_keys input
+    = from_state_alt
+        (cipher state_alt key
+                (fun st k => to_state_alt (add_round_key (from_state_alt st) k))
+                (fun st => to_state_alt (sub_bytes (from_state_alt st)))
+                (fun st => to_state_alt (shift_rows (from_state_alt st)))
+                (fun st => to_state_alt (mix_columns (from_state_alt st)))
+                first_key last_key middle_keys (to_state_alt input)).
+  Proof.
+    intros; subst; cbv [cipher].
+    rewrite !from_state_alt_to_state_alt.
+    repeat (f_equal; [ ]).
+    factor_out_loops.
+    eapply fold_left_double_invariant
+      with (I:=fun b c => c = from_state_alt b);
+      intros; subst;
+        rewrite ?from_state_alt_to_state_alt;
+        reflexivity.
+  Qed.
+
+  Lemma equivalent_inverse_cipher_change_state_rep first_key last_key middle_keys
+        input :
+    equivalent_inverse_cipher
+      state key add_round_key inv_sub_bytes inv_shift_rows inv_mix_columns
+      first_key last_key middle_keys input
+    = from_state_alt
+        (equivalent_inverse_cipher
+           state_alt key
+           (fun st k => to_state_alt (add_round_key (from_state_alt st) k))
+           (fun st => to_state_alt (inv_sub_bytes (from_state_alt st)))
+           (fun st => to_state_alt (inv_shift_rows (from_state_alt st)))
+           (fun st => to_state_alt (inv_mix_columns (from_state_alt st)))
+           first_key last_key middle_keys (to_state_alt input)).
+  Proof.
+    intros; subst; cbv [equivalent_inverse_cipher].
+    rewrite !from_state_alt_to_state_alt.
+    repeat (f_equal; [ ]).
+    factor_out_loops.
+    eapply fold_left_double_invariant
+      with (I:=fun b c => c = from_state_alt b);
+      intros; subst;
+        rewrite ?from_state_alt_to_state_alt;
+        reflexivity.
+  Qed.
+End ChangeRepresentation.
+
+Section Extensionality.
+  Context (state key : Type)
+          (add_round_key add_round_key' : state -> key -> state)
+          (sub_bytes shift_rows mix_columns : state -> state)
+          (sub_bytes' shift_rows' mix_columns' : state -> state)
+          (inv_sub_bytes inv_shift_rows inv_mix_columns : state -> state)
+          (inv_sub_bytes' inv_shift_rows' inv_mix_columns' : state -> state).
+  Context (add_round_key_equiv : forall st k, add_round_key st k = add_round_key' st k)
+          (sub_bytes_equiv : forall st, sub_bytes st = sub_bytes' st)
+          (shift_rows_equiv : forall st, shift_rows st = shift_rows' st)
+          (mix_columns_equiv : forall st, mix_columns st = mix_columns' st)
+          (inv_sub_bytes_equiv : forall st, inv_sub_bytes st = inv_sub_bytes' st)
+          (inv_shift_rows_equiv : forall st, inv_shift_rows st = inv_shift_rows' st)
+          (inv_mix_columns_equiv : forall st, inv_mix_columns st = inv_mix_columns' st).
+
+  Hint Rewrite add_round_key_equiv sub_bytes_equiv shift_rows_equiv mix_columns_equiv
+       inv_sub_bytes_equiv inv_shift_rows_equiv inv_mix_columns_equiv : equiv.
+
+  Lemma cipher_subroutine_ext first_key last_key middle_keys input :
+    cipher state key add_round_key sub_bytes shift_rows mix_columns
+           first_key last_key middle_keys input
+    = cipher state key add_round_key' sub_bytes' shift_rows' mix_columns'
+             first_key last_key middle_keys input.
+  Proof.
+    cbv [cipher]. autorewrite with equiv.
+    erewrite fold_left_ext; [ reflexivity | ].
+    intros. autorewrite with equiv. reflexivity.
+  Qed.
+
+  Lemma equivalent_inverse_cipher_subroutine_ext
+        first_key last_key middle_keys input :
+    equivalent_inverse_cipher
+      state key add_round_key inv_sub_bytes inv_shift_rows inv_mix_columns
+      first_key last_key middle_keys input
+    = equivalent_inverse_cipher
+        state key add_round_key' inv_sub_bytes' inv_shift_rows' inv_mix_columns'
+        first_key last_key middle_keys input.
+  Proof.
+    cbv [equivalent_inverse_cipher]. autorewrite with equiv.
+    erewrite fold_left_ext; [ reflexivity | ].
+    intros. autorewrite with equiv. reflexivity.
+  Qed.
+
+End Extensionality.
